added intt spec and goal tweaks

common/mlkem_mldsa.ml
@@ -111,9 +111,31 @@ let AVX2_REORDER_INVOLUTION = prove
 (* AVX2-optimized ordering for ML-DSA NTT (swaps bit fields then reverses)   *)
 (* ------------------------------------------------------------------------- *)
 
+let bitmap = define
+ `bitmap [] n = 0 /\
+  bitmap (CONS i t) n = bitval(numbit i n) + 2 * bitmap t n`;;
+
 let mldsa_avx2_ntt_order = define
  `mldsa_avx2_ntt_order i =
     bitreverse8(64 * (i DIV 64) + ((i MOD 64) DIV 8) + 8 * (i MOD 8))`;;
+
+let BITMAP_MLDSA_AVX2_NTT_ORDER = prove
+ (`!n. n < 256 ==> bitmap [7;6;2;1;0;5;4;3] n = mldsa_avx2_ntt_order n`,
+  REWRITE_TAC[bitmap; numbit; mldsa_avx2_ntt_order; bitreverse8; bitval] THEN
+  CONV_TAC EXPAND_CASES_CONV THEN
+  CONV_TAC(DEPTH_CONV WORD_NUM_RED_CONV));;
+
+let mldsa_avx2_ntt_order' = define
+ `mldsa_avx2_ntt_order' = bitmap [4;3;2;7;6;5;1;0]`;;
+
+let AVX2_NTT_ORDER_INVOLUTION = prove
+ (`!n. n < 256 ==> mldsa_avx2_ntt_order'(mldsa_avx2_ntt_order n) = n /\
+                   mldsa_avx2_ntt_order(mldsa_avx2_ntt_order' n) = n`,
+  CONV_TAC EXPAND_CASES_CONV THEN
+  REWRITE_TAC[mldsa_avx2_ntt_order; mldsa_avx2_ntt_order'] THEN
+  REWRITE_TAC[bitreverse8; bitmap; bitval; numbit] THEN
+  CONV_TAC(TOP_DEPTH_CONV let_CONV) THEN
+  CONV_TAC(DEPTH_CONV WORD_NUM_RED_CONV));;
 
 (* ------------------------------------------------------------------------- *)
 (* Conversion of each element of an array to Montgomery form with B = 2^16.  *)
@@ -180,7 +202,7 @@ let mldsa_inverse_ntt = define
  `mldsa_inverse_ntt f k =
     (&8347681 * isum (0..255)
                  (\j. f j *
-                      &8347681 pow ((2 * j + 1) * mldsa_avx2_ntt_order k)))
+                      &731434 pow ((2 * j + 1) * mldsa_avx2_ntt_order' k)))
     rem &8380417`;;
 
 (* ------------------------------------------------------------------------- *)
@@ -232,8 +254,8 @@ let MLDSA_FORWARD_NTT = prove
 let MLDSA_INVERSE_NTT = prove
  (`mldsa_inverse_ntt f k =
    (&8347681 * isum (0..255)
-                 (\j. f j * &8347681 pow ((2 * j + 1) * mldsa_avx2_ntt_order k)))
-    rem &8380417`,
+              (\j. f j * &731434 pow ((2 * j + 1) * mldsa_avx2_ntt_order' k)))
+   rem &8380417`,
   REWRITE_TAC[mldsa_inverse_ntt]);;
 
 (* ------------------------------------------------------------------------- *)
@@ -373,9 +395,16 @@ let BITREVERSE8_CLAUSES = end_itlist CONJ (map
  (map (curry mk_comb `bitreverse8` o mk_small_numeral) (0--255)));;
 
 let MLDSA_AVX2_NTT_ORDER_CLAUSES = end_itlist CONJ (map
- (GEN_REWRITE_CONV I [mldsa_avx2_ntt_order] THENC DEPTH_CONV WORD_NUM_RED_CONV THENC
+ (GEN_REWRITE_CONV I [mldsa_avx2_ntt_order] THENC
+  DEPTH_CONV WORD_NUM_RED_CONV THENC
   GEN_REWRITE_CONV I [BITREVERSE8_CLAUSES])
  (map (curry mk_comb `mldsa_avx2_ntt_order` o mk_small_numeral) (0--255)));;
+
+let MLDSA_AVX2_NTT_ORDER_CLAUSES' = end_itlist CONJ (map
+ (GEN_REWRITE_CONV RATOR_CONV [mldsa_avx2_ntt_order'] THENC
+  GEN_REWRITE_CONV TOP_DEPTH_CONV [bitval; numbit; bitmap] THENC
+  DEPTH_CONV WORD_NUM_RED_CONV)
+ (map (curry mk_comb `mldsa_avx2_ntt_order'` o mk_small_numeral) (0--255)));;
 
 let MLDSA_FORWARD_NTT_ALT = prove
  (`mldsa_forward_ntt f k =
@@ -407,7 +436,7 @@ let MLDSA_INVERSE_NTT_ALT = prove
    isum (0..255)
         (\j. f j *
              (&8347681 *
-              (&8347681 pow ((2 * j + 1) * mldsa_avx2_ntt_order k)) rem &8380417)
+           (&731434 pow ((2 * j + 1) * mldsa_avx2_ntt_order' k)) rem &8380417)
              rem &8380417)
     rem &8380417`,
   REWRITE_TAC[mldsa_inverse_ntt; GSYM ISUM_LMUL] THEN
@@ -424,7 +453,7 @@ let MLDSA_INVERSE_NTT_CONV =
   GEN_REWRITE_CONV I [MLDSA_INVERSE_NTT_ALT] THENC
   LAND_CONV EXPAND_ISUM_CONV THENC
   DEPTH_CONV NUM_RED_CONV THENC
-  GEN_REWRITE_CONV ONCE_DEPTH_CONV [MLDSA_AVX2_NTT_ORDER_CLAUSES] THENC
+  GEN_REWRITE_CONV ONCE_DEPTH_CONV [MLDSA_AVX2_NTT_ORDER_CLAUSES'] THENC
   DEPTH_CONV NUM_RED_CONV THENC
   GEN_REWRITE_CONV DEPTH_CONV [INT_OF_NUM_POW; INT_OF_NUM_REM] THENC
   ONCE_DEPTH_CONV EXP_MOD_CONV THENC INT_REDUCE_CONV;;
